
-- --------------------------------------------------------------------------

-- Deduction theorem

dedโโฟ : โ{A B n m} {๐ฑ : Vars n} {๐ญ : Tms n} {ฮ : Cx m}
      โ ฮ , ๐ฃโฟ ๐ฑ โถ A โข *โฟ ๐ญ โถ B
      โ ฮ โข ๐โฟ ๐ฑ ยท ๐ญ โถ (A โ B)
dedโโฟ {๐ฑ = ๐ฑ} {๐ญ = ๐ญ} = M๐โฟ {๐ฑ = ๐ฑ} {๐ญ = ๐ญ}


dedโโฐ : โ{A B m} {ฮ : Cx m}
      โ ฮ โข A โ B
      โ ฮ , A โข B
dedโโฐ D = Mโโฐ (wkโข (drop ฮโฒฮ) D) (M๐ฃโฐ Z)


{-
fooยน : โ{A B x t m} {ฮ : Cx m}
     โ ฮ โข ๐ x ยท t โถ (A โ B)
     โ ฮ , ๐ฃ x โถ A โข ๐ x ยท t โถ (A โ B)
fooยน D = wkโข (drop ฮโฒฮ) D


barยน : โ{A x m} {ฮ : Cx m}
     โ ฮ , ๐ฃ x โถ A โข ๐ฃ x โถ A
barยน = M๐ฃ Z


dedโยน : โ{A B x t m} {ฮ : Cx m}
      โ ฮ โข ๐ x ยท t โถ (A โ B)
      โ ฮ , ๐ฃ x โถ A โข t โถ B
dedโยน D = Mโ (fooยน D) barยน


fooโฟ : โ{A B n m} {๐ฑ : Vars n} {๐ญ : Tms n} {ฮ : Cx m}
     โ ฮ โข ๐โฟ ๐ฑ ยท ๐ญ โถ (A โ B)
     โ ฮ , ๐ฃโฟ ๐ฑ โถ A โข ๐โฟ ๐ฑ ยท ๐ญ โถ (A โ B)
fooโฟ {๐ญ = ๐ญ} D = wkโข (drop ฮโฒฮ) D


barโฟ : โ{A n m} {๐ฑ : Vars n} {ฮ : Cx m}
     โ ฮ , ๐ฃโฟ ๐ฑ โถ A โข ๐ฃโฟ ๐ฑ โถ A
barโฟ {๐ฑ = ๐ฑ} = M๐ฃโฟ {๐ฑ = ๐ฑ} Z


dedโโฟ : โ{A B n m} {๐ฑ : Vars n} {๐ญ : Tms n} {ฮ : Cx m}
      โ ฮ โข ๐โฟ ๐ฑ ยท ๐ญ โถ (A โ B)
      โ ฮ , ๐ฃโฟ ๐ฑ โถ A โข *โฟ ๐ญ โถ B
dedโโฟ {๐ฑ = ๐ฑ} {๐ญ = ๐ญ} D = Mโโฟ (fooโฟ {๐ฑ = ๐ฑ} {๐ญ = ๐ญ} D) (barโฟ {๐ฑ = ๐ฑ})  -- XXX: Prove this!
-}
