module IPC.Hilbert.TreeWithContext.KripkeSoundness where

open import IPC.Hilbert.TreeWithContext public
open import IPC.KripkeSemantics public




-- Using CPS forcing, following Ilik.

module IlikSoundness where
  open IlikSemantics public


  -- FIXME: Add more CPS combinators.
  postulate
    oops : ∀ {A : Set} → A


  -- Soundness, or evaluation.

  eval : ∀ {A Γ} → Γ ⊢ A → Γ ᴹ⊩ A
  eval (var i)             γ = lookup i γ
  eval (app {A} {B} t u)   γ = bind {A ▻ B} {B} (eval t γ)
                                 (λ ξ f → f refl≤ (mono⊩ {A} ξ (eval u γ)))
  eval (ci {A})            γ = return {A ▻ A} (λ _ a → a)
  eval (ck {A} {B})        γ = return {A ▻ B ▻ A} (λ _ a →
                               return {B ▻ A} (λ ξ b → mono⊩ {A} ξ a))
  eval (cs {A} {B} {C})    γ = return {(A ▻ B ▻ C) ▻ (A ▻ B) ▻ A ▻ C} (λ _ f →
                               return {(A ▻ B) ▻ A ▻ C} (λ ξ g →
                               return {A ▻ C} (λ ξ′ t →
                               let f′ = mono⊩ {A ▻ B ▻ C} (trans≤ ξ ξ′) f
                                   g′ = mono⊩ {A ▻ B} ξ′ g
                               in  bind {A} {C} t (λ ξ″ a →
                                   oops))))
  eval (cpair {A} {B})     γ = return {A ▻ B ▻ A ∧ B} (λ _ a →
                               return {B ▻ A ∧ B} (λ ξ b →
                               return {A ∧ B} (mono⊩ {A} ξ a , b)))
  eval (cfst {A} {B})      γ = return {A ∧ B ▻ A} (λ _ t →
                               bind {A ∧ B} {A} t (λ _ s → π₁ s))
  eval (csnd {A} {B})      γ = return {A ∧ B ▻ B} (λ _ t →
                               bind {A ∧ B} {B} t (λ _ s → π₂ s))
  eval tt                  γ = return {⊤} ∙
  eval (cboom {C})         γ = return {⊥ ▻ C} (λ _ t →
                               bind {⊥} {C} t (λ ξ s → elim𝟘 s))
  eval (cinl {A} {B})      γ = return {A ▻ A ∨ B} (λ _ a →
                               return {A ∨ B} (ι₁ a))
  eval (cinr {A} {B})      γ = return {B ▻ A ∨ B} (λ _ b →
                               return {A ∨ B} (ι₂ b))
  eval (ccase {A} {B} {C}) γ = return {A ∨ B ▻ (A ▻ C) ▻ (B ▻ C) ▻ C} (λ _ t →
                               return {(A ▻ C) ▻ (B ▻ C) ▻ C} (λ ξ u →
                               return {(B ▻ C) ▻ C} (λ ξ′ v →
                               let t′ = mono⊩ {A ∨ B} (trans≤ ξ ξ′) t
                                   u′ = mono⊩ {A ▻ C} ξ′ u
                               in  bind {A ∨ B} {C} t′ (λ ξ″ s →
                                   let u″ = mono⊩ {A ▻ C} ξ″ u′
                                       v″ = mono⊩ {B ▻ C} ξ″ v
                                   in elim⊎ s
                                        (λ a → oops)
                                        (λ b → oops)))))
